RCCBase.v
@@ -189,3 +189,71 @@ Coercion comparison2bool : comparison >-> bool.
 Definition bool2Prop (b : bool) : Prop := b = true.
 
 Coercion bool2Prop : bool >-> Sortclass.
+
+(* A way to specify functions that return [comparison]. *)
+Inductive Reflect_cmp (P Q R : Prop) : comparison -> Prop :=
+    | Reflect_Lt : P -> Reflect_cmp P Q R Lt
+    | Reflect_Eq : Q -> Reflect_cmp P Q R Eq
+    | Reflect_Gt : R -> Reflect_cmp P Q R Gt.
+
+Class cmp_spec (A : Type) : Type :=
+{
+    cmpr      : A -> A -> comparison;
+    cmpr_spec :
+      forall x y : A, Reflect_cmp (cmpr y x = Gt) (x = y) (cmpr y x = Lt) (cmpr x y);
+    cmp_spec1 :
+      forall x y : A, cmpr x y = Eq -> x = y;
+    cmp_spec2 :
+      forall x y : A, cmpr x y = Lt <-> cmpr y x = Gt;
+    cmp_spec3 :
+      forall x : A, cmpr x x = Eq;
+}.
+
+Coercion cmpr : cmp_spec >-> Funclass.
+
+Lemma cmp_spec_antirefl :
+  forall {A : Type} (cmp : A -> A -> comparison),
+    (forall x y : A, Reflect_cmp (cmp y x = Gt) (x = y) (cmp y x = Lt) (cmp x y)) ->
+      forall x : A, cmp x x = Lt -> False.
+Proof.
+  intros. specialize (H x x). inv H.
+Qed.
+
+Lemma cmp_spec_asym :
+  forall {A : Type} (cmp : A -> A -> comparison),
+    (forall x y : A, Reflect_cmp (cmp y x = Gt) (x = y) (cmp y x = Lt) (cmp x y)) ->
+      forall x y : A, cmp x y = Lt -> cmp y x <> Lt.
+Proof.
+  intros. specialize (H x y). inv H.
+Qed.
+
+Lemma cmp_spec_trans :
+  forall {A : Type} (cmp : A -> A -> comparison),
+    (forall x y : A, Reflect_cmp (cmp y x = Gt) (x = y) (cmp y x = Lt) (cmp x y)) ->
+      forall x y z : A, cmp x y = Lt -> cmp y z = Lt -> cmp x z = Lt.
+Proof.
+  intros A cmp H x y z Hxy Hyz.
+  pose (H' := H x z). inv H'.
+    pose (H' := H y z). inv H'.
+(*    pose (H' := H y z). inv H'.*)
+Abort.
+
+Lemma cmp_spec_comparison :
+  forall {A : Type} (cmp : A -> A -> comparison),
+    (forall x y : A, Reflect_cmp (cmp y x = Gt) (x = y) (cmp y x = Lt) (cmp x y)) ->
+      forall x y z : A, cmp x z = Lt -> cmp x y = Lt \/ cmp y z = Lt.
+Proof.
+  intros A cmp H x y z Hxz.
+  pose (H' := H x y). inv H'. right.
+  pose (H' := H y z). inv H'.
+  pose (H' := H x z). inv H'.
+Abort.
+
+Lemma cmp_spec_connectedness :
+  forall {A : Type} (cmp : A -> A -> comparison),
+    (forall x y : A, Reflect_cmp (cmp y x = Gt) (x = y) (cmp y x = Lt) (cmp x y)) ->
+      forall x y : A, cmp x y <> Lt -> cmp y x <> Lt -> cmp x y = Eq.
+Proof.
+  intros A cmp H x y Hxy Hyx.
+  pose (H' := H x y). inv H'.
+Qed.
