Sorting/TreeSort.v
@@ -6,73 +6,115 @@ Require Export BST.
 
 Require Export ListLemmas.
 
+Fixpoint insertBT {A : Type} (cmp : A -> A -> bool) (x : A) (t : BTree A) : BTree A :=
+match t with
+    | empty => node x empty empty
+    | node v l r =>
+        if cmp x v
+        then node v (insertBT cmp x l) r
+        else node v l (insertBT cmp x r)
+end.
+
+Fixpoint fromList
+  {A : Type} (cmp : A -> A -> bool) (l : list A) : BTree A :=
+match l with
+    | [] => empty
+    | h :: t => insertBT cmp h (fromList cmp t)
+end.
+
 Definition treeSort
-  {A : Type} (cmp : A -> A -> comparison) (l : list A) : list A :=
+  {A : Type} (cmp : A -> A -> bool) (l : list A) : list A :=
     BTree_toList (fromList cmp l).
 
+Lemma Elem_insertBT :
+  forall {A : Type} (cmp : A -> A -> comparison) (x y : A) (t : BTree A),
+    Elem x (insertBT cmp y t) -> cmp x y = Eq \/ Elem x t.
+Proof.
+Admitted.
+
+Lemma isBST_insertBT :
+  forall {A : Type} (cmp :  A -> A -> comparison) (x : A) (t : BTree A),
+    isBST cmp t -> isBST cmp (insertBT cmp x t).
+Proof.
+  induction t as [| v l IHl r IHr]; cbn.
+    auto.
+    intro. destruct (cmp x v) eqn: Hcmp; cbn; auto.
+      inv H. constructor; auto. intros. apply Elem_insertBT in H. destruct H; auto.
+Admitted.
+
+(* Lemma count_BTree_insert :
+  forall (A : Type) (cmp : cmp_spec A) (p : A -> bool) (x : A) (t : BTree A),
+    count_BTree p (insert cmp x t) =
+      if p x then 1 + count_BTree p t else count_BTree p t.
+Proof.
+  induction t; cbn.
+    reflexivity.
+    destruct (cmpr_spec x a); cbn;
+      rewrite ?IHt1, ?IHt2;
+      destruct (p x) eqn: Hpx, (p a) eqn: Hpa; cbn; try lia.
+Abort.
+ *)
+
+Lemma isBST_fromList :
+  forall {A : Type} (cmp : A -> A -> comparison) (l : list A),
+    isBST cmp (fromList cmp l).
+Proof.
+  induction l as [| h t]; cbn.
+    constructor.
+    apply isBST_insertBT. assumption.
+Qed.
+
 Lemma Sorted_treeSort :
-  forall (A : Type) (cmp : cmp_spec A) (l : list A),
-    Sorted cmpr (treeSort cmp l).
+  forall {A : Type} (cmp : A -> A -> comparison) (l : list A),
+    Sorted cmp (treeSort cmp l).
 Proof.
   unfold treeSort. intros. apply Sorted_BTree_toList, isBST_fromList.
 Qed.
 
-Lemma perm_treeSort :
-  forall (A : Type) (cmp : A -> A -> comparison) (l : list A),
-    perm (treeSort cmp l) l.
-Proof.
-  induction l as [| h t]; intro; cbn.
-    reflexivity. Search count insert.
-    rewrite count_toList. Search count_BTree. count_BTree_insert, <- count_toList, <- IHt. reflexivity.
-Qed.
-
-Lemma Permutation_treeSort_aux :
-  forall (A : LinDec) (x : A) (t : BTree A),
-    Permutation (BTree_toList (BTree_ins x t)) (x :: BTree_toList t).
+Lemma count_BTree_insertBT :
+  forall {A : Type} (cmp : A -> A -> bool) (p : A -> bool) (x : A) (t : BTree A),
+    count_BTree p (insertBT cmp x t) =
+      if p x then 1 + count_BTree p t else count_BTree p t.
 Proof.
   induction t as [| v l r]; cbn.
     reflexivity.
-    destruct (x <=? v); cbn.
+    destruct (cmp x v); cbn; destruct (p v), (p x); lia.
+Qed.
+
+Lemma perm_treeSort :
+  forall {A : Type} (cmp : A -> A -> bool) (l : list A),
+    perm (treeSort cmp l) l.
+Proof.
+  induction l as [| h t]; intro; cbn.
+    reflexivity.
+    rewrite count_toList, count_BTree_insertBT, <- count_toList, <- IHt. reflexivity.
+Qed.
+
+Lemma Permutation_treeSort_aux :
+  forall {A : Type} (cmp : A -> A -> bool) (x : A) (t : BTree A),
+    Permutation (BTree_toList (insertBT cmp x t)) (x :: BTree_toList t).
+Proof.
+  induction t as [| v l r]; cbn.
+    reflexivity.
+    destruct (cmp x v); cbn.
       rewrite r. cbn. reflexivity.
-      rewrite IHt1. rewrite Permutation_app_comm, perm_swap. cbn.
+      rewrite IHt1, Permutation_app_comm, perm_swap. cbn.
         constructor. rewrite Permutation_app_comm, Permutation_middle.
           reflexivity.
 Qed.
 
 Lemma Permutation_treeSort :
-  forall (A : LinDec) (l : list A),
-    Permutation (treeSort A l) l.
+  forall {A : Type} (cmp : A -> A -> bool) (l : list A),
+    Permutation (treeSort cmp l) l.
 Proof.
   induction l as [| h t]; cbn.
     reflexivity.
     rewrite Permutation_treeSort_aux. constructor. assumption.
 Qed.
 
-#[refine]
-Instance Sort_treeSort (A : LinDec) : Sort A :=
+Instance Sort_treeSort (A : Type) (cmp : A -> A -> comparison) : Sort cmp :=
 {
-    sort := @treeSort A;
-    Sorted_sort := Sorted_treeSort A;
+    sort := treeSort cmp;
+    Sorted_sort := Sorted_treeSort cmp;
+    Permutation_sort := Permutation_treeSort cmp;
 }.
-Proof.
-  intros. apply perm_Permutation. rewrite <- perm_treeSort. reflexivity.
-Defined.
-
-Lemma treeSort'_spec :
-  @treeSort' = @treeSort.
-Proof.
-  ext A. ext l. unfold treeSort'.
-  rewrite fromList'_spec, BTree_toList'_spec.
-  unfold treeSort. reflexivity.
-Qed.
-
-#[refine]
-Instance Sort_treeSort' (A : LinDec) : Sort A :=
-{
-    sort := @treeSort' A;
-}.
-Proof.
-  all: intros; rewrite treeSort'_spec.
-    apply Sorted_treeSort.
-    apply perm_Permutation. rewrite <- perm_treeSort. reflexivity.
-Defined.
